Hoare/TrTermination.thy
@@ -986,5 +986,21 @@ using next_state_gas_continue apply force
 using next_state_gas_env apply force
 done
 
+fun iter_next :: "network \<Rightarrow> global_state \<Rightarrow> nat \<Rightarrow> global_state" where
+"iter_next net g 0 = g"
+| "iter_next net g (Suc n) = iter_next net (next0 net g) n"
+
+fun seq_next :: "network \<Rightarrow> global_state \<Rightarrow> nat \<Rightarrow> global_state list" where
+"seq_next net g 0 = [g]"
+| "seq_next net g (Suc n) = g # seq_next net (next0 net g) n"
+
+lemma seq_next_nil : "seq_next net g n = [] \<Longrightarrow> False"
+by (cases n, auto)
+
+lemma iter_seq : "last (seq_next net g n) = iter_next net g n"
+apply (induction n arbitrary:g, auto)
+using seq_next_nil apply force
+done
+
 end
 
