Hoare/Invariants.thy
@@ -1,0 +1,71 @@
+theory Invariants
+imports "TrTermination"
+begin
+
+definition basic_inv :: "global0 \<Rightarrow> bool" where
+"basic_inv g = (memu_invariant g \<and> gas_invariant g \<and>
+   total_balance (g_orig g) < 2^256 \<and> balance_inv g)"
+
+lemma orig_balance :
+  "total_balance (g_orig g) < 2^256 \<Longrightarrow>
+   balance_inv g \<Longrightarrow>
+   total_balance (g_current g) < 2^256"
+  using inv_orig_current by fastforce
+
+
+lemma basic_invariant :
+  "Continue st2 = next0 net (Continue st1) \<Longrightarrow>
+   basic_inv st1 \<Longrightarrow>
+   basic_inv st2"
+  by (metis basic_inv_def gas_next memu_next orig_balance tr_balance_continue tr_orig)
+
+definition re_invariant ::
+   "global0 \<Rightarrow> address \<Rightarrow> (w256 \<Rightarrow> storage \<Rightarrow> bool) \<Rightarrow> bool" where
+"re_invariant g addr iv = (
+  iv (account_balance0 (g_current g addr))
+     (account_storage0 (g_current g addr)) \<and>
+  (\<forall>x y s. iv x s \<longrightarrow> x < y \<longrightarrow> iv y s))"
+
+definition pop_action :: "contract_action \<Rightarrow> bool" where
+"pop_action act =
+   (act \<in> range ContractFail \<union> range ContractSuicide
+            \<union> range ContractReturn)"
+
+definition re_assumption ::
+  "network \<Rightarrow> address \<Rightarrow> program \<Rightarrow> (w256 \<Rightarrow> storage \<Rightarrow> bool) \<Rightarrow> bool" where
+"re_assumption net addr prog iv =
+  (\<forall>g args v1 h1.
+      g_vmstate g = InstructionToEnvironment (ContractCall args) v1 h1 \<longrightarrow>
+      callarg_recipient args = addr \<longrightarrow>
+      account_code0 (g_current g addr) = prog \<longrightarrow>
+  (\<exists>k g1 g2 g3 act2 v2 h2.
+      Unimplemented = iter_next net (Continue g) k \<or>
+      Continue g1 = next0 net (Continue g) \<and>
+      Continue g2 = iter_next net (Continue g) k \<and>
+      Continue g3 = iter_next net (Continue g) (Suc k) \<and>
+      g_vmstate g2 = InstructionToEnvironment act2 v2 h2 \<and>
+      pop_action act2 \<and>
+      g_stack g2 = g_stack g1 \<and>
+      re_invariant g3 addr iv))"
+
+(* call stack changes *)
+
+lemma stack_changes :
+  "Continue st2 = next0 net (Continue st1) \<Longrightarrow>
+   g_stack st2 = g_stack st1 \<or>
+   g_stack st2 = tl (g_stack st1) \<or>
+   tl (g_stack st2) = g_stack st1"
+by (auto simp add:next0_def Let_def
+  split:if_split_asm option.split_asm list.split_asm
+   contract_action.split_asm stack_hint.split_asm
+   instruction_result.splits)
+
+(* storage changes *)
+
+(* code changes *)
+
+(* balance changes *)
+
+end
+
+
